src/tools/parallelcomposition/translateTosapic/translate_to_sapicScript.sml
@@ -8,11 +8,13 @@ open Arbnumcore;
 open bir_immTheory;
 open integerTheory;
 open Term;
+open sbir_treeTheory;
 
 
 
 val _ = new_theory "translate_to_sapic";                
 
+(*****************start translation Bir Exp to Sapic Term**********************)
 
 val translate_Imm_to_string_def = Define`
 translate_Imm_to_string imm =
@@ -20,14 +22,17 @@ translate_Imm_to_string imm =
 
 `;
 
-val translate_imm_to_sapic_term_def = Define`
-translate_imm_to_sapic_term imm =
-Con (Name PubName ((toString o b2n) imm))
 
-`;
+ val translate_birvar_to_sapicterm_def = Define`
+ translate_birvar_to_sapicterm (BVar str (BType_Imm s)) =
+ TVar (Var str ((int_of_num o size_of_bir_immtype) s))
+      `;
 
-
-    
+ val translate_bir_immtype_to_sapicterm_def = Define`
+ translate_bir_immtype_to_sapicterm immty =
+ Con (Name PubName ((toString o size_of_bir_immtype) immty))
+      `;        
+      
 val translate_UnaryExp_to_string_def = Define`
 translate_UnaryExp_to_string ue =
 (case ue of
@@ -85,4 +90,48 @@ translate_Endian_to_string en =
  | BEnd_NoEndian     => "NoEndian"
 )`;
 
+
+val translate_birexp_to_sapicterm_def = Define`
+                                               translate_birexp_to_sapicterm exp =
+ (case exp of
+    BExp_Const c                      => Con (Name PubName (translate_Imm_to_string c))
+  | BExp_MemConst v1 v2 v3            => Con (Name PubName (toString ((size_of_bir_immtype v1) + (size_of_bir_immtype v2))))
+  | BExp_Den (BVar str _)             => TVar (Var str 0)
+  | BExp_Load e1 e2 a b               => FAPP ("Load",(2, Public, Constructor)) [(translate_birexp_to_sapicterm e1);(translate_birexp_to_sapicterm e2)]
+  | BExp_Store e1 e2 a e3             => FAPP ("Store",(3, Public, Destructor)) [(translate_birexp_to_sapicterm e1);(translate_birexp_to_sapicterm e2);(translate_birexp_to_sapicterm e3)]
+  | BExp_UnaryExp ue e                => FAPP ((translate_UnaryExp_to_string ue),(1, Public, Constructor)) [(translate_birexp_to_sapicterm e)]
+  | BExp_BinExp be e1 e2              => FAPP ((translate_BinExp_to_string be),(2, Public, Constructor)) [(translate_birexp_to_sapicterm e1);(translate_birexp_to_sapicterm e2)]
+  | BExp_BinPred bp e1 e2             => FAPP ((translate_BinPred_to_string bp),(2, Public, Constructor)) [(translate_birexp_to_sapicterm e1);(translate_birexp_to_sapicterm e2)]
+  | BExp_MemEq e1 e2                  => FAPP ("MemEq",(2, Public, Constructor)) [(translate_birexp_to_sapicterm e1);(translate_birexp_to_sapicterm e2)]
+  | BExp_IfThenElse e1 e2 e3          => FAPP ("IfThenElse",(3, Public, Destructor)) [(translate_birexp_to_sapicterm e1);(translate_birexp_to_sapicterm e2);(translate_birexp_to_sapicterm e3)]
+  | BExp_Cast v8 v9 v10               => FAPP ((translate_Cast_to_string v8),(2, Public, Constructor)) [(translate_birexp_to_sapicterm v9);(Con (Name PubName ((toString o size_of_bir_immtype) v10)))]
+ ) 
+ `;
+
+        
+(*****************end translation Bir Exp to Sapic Term**********************)
+(*
+                      
+val tree_node_to_process_thm = store_thm(
+  "tree_node_to_process",
+        ``∀(Tree: bir_exp_t stree) (var: bir_exp_t) (valu: bir_exp_t). ((var,valu) ∈ (STATES Tree)) ⇒ (∃(C:sapic_configuration_t). THE (sapic_substitution_get (get_substitution_conf C) (THE ( var_of_term (translate_birexp_to_sapicterm var)))) = (translate_birexp_to_sapicterm valu))``,
+                           rpt strip_tac >>
+                           Q.EXISTS_TAC `Config (Ns,St,Pold,(Substitution Sb),Al)`>>
+                       rewrite_tac[sapic_substitution_get_def,get_substitution_conf_def] >>
+                       Cases_on `var` >>
+                       rewrite_tac[translate_birexp_to_sapicterm_def]
+
+                        
+  );
+
+translate_birexp_to_sapicterm (BExp_Const (Imm64 64w)) = Con (Name PubName "64")
+
+  val sim_def = Define`
+sim sbst spcf  =
+(
+)`; 
+*)
+
+       
+  
 val _ = export_theory();
